extend simpl and add forall+biab tactic

shiftreset/Mechanized/State.v
@@ -4,6 +4,84 @@
 From Stdlib Require Import Classes.RelationClasses.
 From ShiftReset Require Import Logic Automation Entl Norm Propriety.
 
+#[global]
+Instance Proper_pointwise_eq_ens : Proper (Morphisms.pointwise_relation val eq ====> entails) ens.
+Proof.
+  unfold Proper, respectful, Morphisms.pointwise_relation, entails. intros.
+  inverts H0.
+  destruct H7 as (v&h3&P&Q&S&T). subst. apply s_ens.
+  eexists. eexists.
+  rewrite <- H.
+  intuition.
+  auto.
+Qed.
+
+#[global]
+Instance Proper_pointwise_himpl_ens : Proper (Morphisms.pointwise_relation val himpl ====> entails) ens.
+Proof.
+  unfold Proper, respectful, Morphisms.pointwise_relation, entails. intros.
+  inverts H0.
+  destruct H7 as (v&h3&P&Q&S&T). subst. apply s_ens.
+  eexists. eexists.
+  intuition.
+  apply H.
+  auto.
+Qed.
+
+#[global]
+Instance Proper_hstar_himpl : Proper (himpl ====> himpl ====> himpl) hstar.
+Proof.
+  unfold Proper, respectful, Morphisms.pointwise_relation, flip. intros.
+  apply (@himpl_trans (y \* x0)); xsimpl; auto.
+Qed.
+
+#[global]
+Instance Proper_qimpl_ens : Proper ((@qimpl val) ====> entails) ens.
+Proof.
+  unfold Proper, respectful, entails. intros * Hqimpl * Hens.
+  inverts Hens. destr H5. subst. constructor. eexists. eexists. intuition. 
+  unfold qimpl, himpl in Hqimpl. auto.
+Qed.
+
+#[global]
+Instance Proper_himpl_ens_void : Proper (himpl ====> entails) ens_.
+Proof.
+  unfold Proper, respectful, entails. intros * Hhimpl * Hens.
+  inverts Hens. destr H5. hinv H0. hinv H0. subst. constructor. eexists. eexists. intuition.
+  hintro.
+  - apply hpure_intro. auto.
+  - apply Hhimpl. auto.
+  - auto.
+Qed.
+
+#[global]
+Instance Proper_himpl_req_void : Proper (flip himpl ====> eq ====> entails) req.
+Proof.
+  unfold Proper, respectful, entails. intros * Hhimpl * H. subst.
+  intros * Hreq.
+  inverts Hreq. 
+  applys* s_req.
+Qed.
+
+Lemma bientails_iff_entails : forall f1 f2,
+  bientails f1 f2 <-> (entails f1 f2 /\ entails f2 f1).
+Proof.
+  unfold bientails, entails.
+  intros. split; intuition; apply H; auto.
+Qed.
+
+
+#[global]
+Instance Proper_pointwise_bientails_fex : forall A,
+  Proper (Morphisms.pointwise_relation A bientails ====> bientails)
+  (@fex A).
+Proof.
+  unfold Proper, respectful, Morphisms.pointwise_relation.
+  intros * Hbient.
+  apply bientails_iff_entails.  
+  split; fdestruct v; fexists v; lets H: Hbient v; apply bientails_iff_entails in H; intuition.
+Qed.
+
 Inductive hpred :=
   | hsplit (lhs : hpred) (rhs : hpred)
   | hpts_to (p : loc) (v : val)
@@ -35,6 +113,50 @@ Inductive precond_reflect : Prop -> hpred -> hprop -> Prop :=
       precond_reflect P1 h1 hp1 ->
       precond_reflect P2 h2 hp2 ->
       precond_reflect (P1 /\ P2) (hsplit h1 h2) (hp1 \* hp2).
+
+Lemma hpure_conj_star_star : forall P1 P2 H1 H2,
+  \[P1 /\ P2] \* H1 \* H2 ==> (\[P1] \* H1) \* (\[P2] \* H2).
+Proof.
+  intros.
+  rewrite <- hstar_hpure_conj.
+  rewrite (hstar_comm H1).
+  rewrite hstar_assoc. 
+  rewrite <- (hstar_assoc \[P2] _ _).
+  rewrite (hstar_comm (_ \* _)).
+  rewrite <- hstar_assoc.
+  apply himpl_refl.
+Qed.
+
+Lemma hpure_conj_star_star_conv : forall P1 P2 H1 H2,
+  (\[P1] \* H1) \* (\[P2] \* H2) ==> \[P1 /\ P2] \* H1 \* H2.
+Proof.
+  intros.
+
+  rewrite <- hstar_hpure_conj.
+  rewrite hstar_assoc. 
+  rewrite <- (hstar_assoc H1 _ _).
+  rewrite (hstar_comm H1).
+  rewrite (hstar_assoc \[P2]).
+  rewrite hstar_assoc.
+  apply himpl_refl.
+Qed.
+
+Lemma precond_reflect_himpl_hprop : forall P h hp,
+  precond_reflect P h hp -> (\[P] \* (hprop_of_hpred h) ==> hp /\ hp ==> \[P] \* (hprop_of_hpred h)).
+Proof.
+  intros * Hrefl.
+  induction Hrefl.
+  - unfold hprop_of_hpred. intuition; xsimpl; auto.
+  - unfold hprop_of_hpred. intuition; xsimpl; auto.
+  - destruct IHHrefl1 as [IH1a IH1b].
+    destruct IHHrefl2 as [IH2a IH2b].
+    simpl. split.
+    + apply (himpl_trans (hpure_conj_star_star _ _ _ _)).
+      apply himpl_frame_lr; assumption.
+    + eapply himpl_trans.
+      apply himpl_frame_lr; [apply IH1b | apply IH2b ].
+      apply hpure_conj_star_star_conv.
+Qed.
 
 Definition postcond_value {A : Type} (v : A) H Q := 
   (Q ===> (fun res => \[res = v] \* H))
@@ -89,14 +211,21 @@ Proof.
   intros. unfold ens_state. reflexivity.
 Qed.
 
+Lemma ens_vunit_is_ens_void : forall H, ens (fun res => \[res = vunit] \* H) = ens_ H.
+Proof.
+  unfold ens_. intros. reflexivity.
+Qed.
+
+
 (* Rewrites all [ens_state]s present in the goal back to an [ens]. *)
   (* TODO [rew_state_to_hprop in H] *)
 Ltac rew_state_to_hprop := 
   unfold ens_pure, ens_heap, ens_ret;
   rewrite ?ens_state_vunit_is_ens_state_void;
   rewrite ?ens_state_void_is_ens_void;
-  unfold ens_state, hprop_of_hpred;
+  unfold ens_state, req_state, hprop_of_hpred;
   (* clean up the postconditions *)
+  rewrite ?ens_vunit_is_ens_void;
   rewrite <- ?hempty_eq_hpure_true;
   autorewrite with rew_heap;
   (*rewrite <- hempty_eq_hpure_true;*)
@@ -106,56 +235,6 @@ Ltac rew_state_to_hprop :=
 (* now we can write a rewriting lemma *)
 
 (* this lets us use SLF's heap rewrite lemmas inside an ens *)
-#[global]
-Instance Proper_pointwise_eq_ens : Proper (Morphisms.pointwise_relation val eq ====> entails) ens.
-Proof.
-  unfold Proper, respectful, Morphisms.pointwise_relation, entails. intros.
-  inverts H0.
-  destruct H7 as (v&h3&P&Q&S&T). subst. apply s_ens.
-  eexists. eexists.
-  rewrite <- H.
-  intuition.
-  auto.
-Qed.
-
-#[global]
-Instance Proper_pointwise_himpl_ens : Proper (Morphisms.pointwise_relation val himpl ====> entails) ens.
-Proof.
-  unfold Proper, respectful, Morphisms.pointwise_relation, entails. intros.
-  inverts H0.
-  destruct H7 as (v&h3&P&Q&S&T). subst. apply s_ens.
-  eexists. eexists.
-  intuition.
-  apply H.
-  auto.
-Qed.
-
-#[global]
-Instance Proper_hstar_himpl : Proper (himpl ====> himpl ====> himpl) hstar.
-Proof.
-  unfold Proper, respectful, Morphisms.pointwise_relation, flip. intros.
-  apply (@himpl_trans (y \* x0)); xsimpl; auto.
-Qed.
-
-#[global]
-Instance Proper_qimpl_ens : Proper ((@qimpl val) ====> entails) ens.
-Proof.
-  unfold Proper, respectful, entails. intros * Hqimpl * Hens.
-  inverts Hens. destr H5. subst. constructor. eexists. eexists. intuition. 
-  unfold qimpl, himpl in Hqimpl. auto.
-Qed.
-
-#[global]
-Instance Proper_himpl_ens_void : Proper (himpl ====> entails) ens_.
-Proof.
-  unfold Proper, respectful, entails. intros * Hhimpl * Hens.
-  inverts Hens. destr H5. hinv H0. hinv H0. subst. constructor. eexists. eexists. intuition.
-  hintro.
-  - apply hpure_intro. auto.
-  - apply Hhimpl. auto.
-  - auto.
-Qed.
-
 Lemma ens_duplicate_pure : forall P,
   bientails (ens (fun r => \[P r])) (ens (fun r => \[P r]) ;; ens (fun r => \[P r])).
 Proof.
@@ -185,10 +264,57 @@ Proof.
     fentailment. xsimpl; intros; intuition.
 Qed.
 
+Lemma norm_combine_ens_void : forall P h Q,
+  precond_reflect P h Q -> entails (ens_state_ P h) (ens_ Q).
+Proof.
+  intros * Hrefl.
+  induction Hrefl; rew_state_to_hprop.
+  - reflexivity.
+  - reflexivity.
+  - apply precond_reflect_himpl_hprop in Hrefl1.
+    apply precond_reflect_himpl_hprop in Hrefl2.
+    destruct Hrefl1 as [Hrefl1 _].
+    destruct Hrefl2 as [Hrefl2 _].
+    apply entl_ens_void_single.
+    apply (himpl_trans (hpure_conj_star_star _ _ _ _)).
+    apply himpl_frame_lr; assumption.
+Qed.
+
 Lemma norm_split_req_void : forall P h Q f,
   precond_reflect P h Q -> entails (req Q f) (req_state P h f).
 Proof.
-Admitted.
+  intros * Hrefl.
+  generalize dependent f.
+  induction Hrefl; rew_state_to_hprop; try (intros; reflexivity).
+  apply precond_reflect_himpl_hprop in Hrefl1.
+  apply precond_reflect_himpl_hprop in Hrefl2.
+  destruct Hrefl1 as [Hrefl1 _].
+  destruct Hrefl2 as [Hrefl2 _].
+  intros.
+  apply entl_req_req.
+  - apply (himpl_trans (hpure_conj_star_star _ _ _ _)).
+    apply himpl_frame_lr; assumption.
+  - reflexivity.
+Qed.
+
+Lemma norm_combine_req_void : forall P h Q f,
+  precond_reflect P h Q -> entails (req_state P h f) (req Q f).
+Proof.
+  intros * Hrefl.
+  generalize dependent f.
+  induction Hrefl; rew_state_to_hprop; try (intros; reflexivity).
+  intros.
+  apply precond_reflect_himpl_hprop in Hrefl1.
+  apply precond_reflect_himpl_hprop in Hrefl2.
+  destruct Hrefl1 as [_ Hrefl1].
+  destruct Hrefl2 as [_ Hrefl2].
+  apply entl_req_req. 2: { reflexivity. }
+  eapply himpl_trans.
+  - apply himpl_frame_lr.
+    + apply Hrefl1.
+    + apply Hrefl2.
+  - apply hpure_conj_star_star_conv.
+Qed.
 
 Lemma norm_split_ens : forall v P h Q,
   postcond_reflect v P h Q -> entails (ens Q) (ens_state P h v).
@@ -204,6 +330,43 @@ Proof.
   rewrite norm_ens_ens_void_l.
   rew_state_to_hprop.
   reflexivity.
+Qed.
+
+Lemma norm_combine_ens : forall v P h Q,
+  postcond_reflect v P h Q -> entails (ens_state P h v) (ens Q).
+Proof.
+  intros * Hrefl.
+  inverts Hrefl.
+  apply norm_combine_ens_void in Hprecond.
+  unfold ens_state.
+  inverts Hvalue.
+  rewrite <- H0.
+  rewrite <- norm_ens_ens_void_l.
+  unfold ens_.
+  unfold ens_state_, ens_state in Hprecond.
+  rewrite Hprecond.
+  rewrite norm_ens_ens_void_l.
+  reflexivity.
+Qed.
+
+Lemma norm_ens_bient_ens_state : forall v P h Q,
+  postcond_reflect v P h Q -> bientails (ens Q) (ens_state P h v).
+Proof.
+  intros * Hrefl.
+  apply bientails_iff_entails.
+  split.
+  - apply norm_split_ens. exact Hrefl.
+  - apply norm_combine_ens. exact Hrefl.
+Qed.
+
+Lemma norm_req_bient_req_state : forall P h Q f,
+  precond_reflect P h Q -> bientails (req Q f) (req_state P h f).
+Proof.
+  intros * Hrefl.
+  apply bientails_iff_entails.
+  split.
+  - apply norm_split_req_void. exact Hrefl.
+  - apply norm_combine_req_void. exact Hrefl.
 Qed.
 
 (* Solves a goal of the form [precond_reflect _ _ Q]. This is most useful when
@@ -253,21 +416,35 @@ End Lock.
 Definition lock := Lock.lock.
 Definition locked := Lock.locked.
 
-Ltac frewrite_ens_to_ens_state_one :=
-  setoid_rewrite norm_split_ens at 1;
-  try match goal with
-  | [ |- postcond_reflect _ _ _ _ ] => 
-      eapply postc_refl_val;
-      [ fsolve_post_value | fsolve_prec_reflect ]
-  end;
-  autorewrite with rew_simpl_pure;
-  (* unlock all ens_state *)
-  try rewrite <- (lock _ ens_state);
+Ltac relock_ens_state := 
   (* lock all ens_states, including the one we just rewrote *)
   (* this is to prevent the setoid_rewrite from rewriting this state,
      since it is also just an ens_ in the background *)
+  try rewrite <- (lock _ ens_state);
   rewrite (lock _ ens_state).
 
+Ltac relock_req_state :=
+  (* lock all ens_states, including the one we just rewrote *)
+  (* this is to prevent the setoid_rewrite from rewriting this state,
+     since it is also just an ens_ in the background *)
+  try rewrite <- (lock _ req_state);
+  rewrite (lock _ req_state).
+
+Ltac frewrite_req_to_req_state_one :=
+  first [ rewrite norm_req_bient_req_state at 1 | setoid_rewrite norm_req_bient_req_state at 1];
+  [ | fsolve_prec_reflect];
+  autorewrite with rew_simpl_pure;
+  relock_req_state.
+
+Ltac frewrite_ens_to_ens_state_one :=
+  first [ rewrite norm_ens_bient_ens_state at 1 | setoid_rewrite norm_ens_bient_ens_state at 1];
+  [ | match goal with
+      | [ |- postcond_reflect _ _ _ _ ] => 
+          eapply postc_refl_val;
+          [ fsolve_post_value | fsolve_prec_reflect ]
+      end];
+  autorewrite with rew_simpl_pure;
+  relock_ens_state.
 
 (* A hack to force Coq to only rewrite the right-hand side of an entailment. *)
 Definition entailsR a b := entails b a.
@@ -280,14 +457,24 @@ Proof. reflexivity. Qed.
 Typeclasses Opaque entailsR.
 
 Instance Proper_entails_entailsR :
-  Proper (flip entails ====> eq ====> impl) entailsR.
+  Proper (entails ====> eq ====> impl) entailsR.
 Proof.
-Admitted.
+  unfold Proper, respectful, entails, entailsR, flip, impl.
+  intros * H * Hx0 Hentx0. subst. fold (entails x y) in H.
+  pose proof entails_trans as Ht. unfold Transitive in Ht.
+  apply (Ht _ x _); auto.
+Qed.
 
 Instance Proper_bientails_entailsR :
   Proper (bientails ====> eq ====> iff) entailsR.
 Proof.
-Admitted.
+  unfold Proper, respectful, entailsR, iff.
+  intros. subst. apply bientails_iff_entails in H. destr H.
+  pose proof entails_trans as Ht. unfold Transitive in Ht.
+  split.
+  - intros Hy. apply (Ht _ x _); auto.
+  - intros Hy. apply (Ht _ y _); auto.
+Qed.
 
 Ltac with_entailsR_base tac :=
   rewrite <- entailsR_is_entails;
@@ -298,8 +485,10 @@ Tactic Notation "with_entailsR" tactic(tac) := with_entailsR_base ltac:(tac).
 
 Ltac rew_hprop_to_state :=
   (* unlock all the ens_states once we are done *)
-  (with_entailsR (repeat frewrite_ens_to_ens_state_one; rewrite <- ?(lock _ ens_state)));
-  (repeat frewrite_ens_to_ens_state_one; rewrite <- ?(lock _ ens_state)).
+  (repeat frewrite_ens_to_ens_state_one);
+  rewrite <- ?(lock _ ens_state);
+  (repeat frewrite_req_to_req_state_one);
+  rewrite <- ?(lock _ req_state).
 
 Lemma norm_seq_ens_ret_ens_pure : 
   forall P v, entails (ens_ret v ;; ens_pure P) (ens_pure P ;; ens_ret v).
@@ -369,13 +558,6 @@ Notation "'let\'' x '=' f1 'in' f2" :=
 
 (* some more Proper instances that should really be in Propriety *)
 
-Lemma bientails_iff_entails : forall f1 f2,
-  bientails f1 f2 <-> (entails f1 f2 /\ entails f2 f1).
-Proof.
-  unfold bientails, entails.
-  intros. split; intuition; apply H; auto.
-Qed.
-
 #[global]
 Instance Proper_pointwise_entails_fex : forall A,
   Proper (Morphisms.pointwise_relation A entails ====> entails)
@@ -394,16 +576,6 @@ Qed.
 (*  (@fex A).*)
 (*Proof.*)
 (*Admitted.*)
-
-#[global]
-Instance ShiftFree_locked_ens : forall P h v,
-  ShiftFree ((Lock.locked _ ens_state) P h v).
-Proof.
-  intros.
-  rewrite <- (lock _ _).
-  constructor.
-  unfold ens_state. shiftfree.
-Qed.
 
 #[global]
 Instance bient_ent_subrelation : subrelation bientails entails.
@@ -440,6 +612,105 @@ Proof.
   - no_shift.
 Qed.
 
+(* we define some typeclasses weaker than ShiftFree, but still allow for nice rewriting properties *)
+(*Class AssociateWithSeq (f : flow) := {*)
+(*  assoc_with_seq_proof : forall f1 fk, bientails (bind (f ;; f1) fk) (f ;; bind f1 fk)*)
+(*}.*)
+(**)
+(*#[global]*)
+(*Instance Associate_with_seq_sf : forall f, ShiftFree f -> AssociateWithSeq f.*)
+(*Proof.*)
+(*Admitted.*)
+
+Class RewritableBinder (f : flow) : Prop := {
+  rewritable_binder_proof : forall f1 f2, (forall v, entails (f1 v) (f2 v)) -> entails (bind f f1) (bind f f2)
+}.
+
+#[global]
+Instance Proper_binder_rewrite : forall f,RewritableBinder f ->
+  Proper (Morphisms.pointwise_relation _ entails ====> entails) (bind f).
+Proof.
+Admitted.
+
+#[global]
+Instance Proper_binder_rewrite_seq : forall f,RewritableBinder f ->
+  Proper (entails ====> entails) (seq f).
+Proof.
+Admitted.
+
+#[global]
+Instance Proper_binder_rewrite_bient_seq : forall f,RewritableBinder f ->
+  Proper (bientails ====> bientails) (seq f).
+Proof.
+Admitted.
+
+#[global]
+Instance Rewrite_binder_sf : forall f, ShiftFree f -> RewritableBinder f.
+Proof.
+Admitted.
+
+#[global]
+Instance Rewrite_locked_ens_state : forall P h v, RewritableBinder ((Lock.locked _ ens_state) P h v).
+Proof.
+  rewrite <- (lock _ ens_state).
+  intros.
+  apply Rewrite_binder_sf.
+  unfold ens_state. constructor. shiftfree.
+Qed.
+
+Lemma norm_bind_req_conv : forall H f fk, entails (req H (bind f fk)) (bind (req H f) fk).
+Proof.
+Admitted.
+
+Lemma norm_bind_all_l_conv : forall A fk1 fk, entails (@fall A (fun b => (bind (fk1 b) fk))) (bind (fall fk1) fk).
+Proof.
+Admitted.
+
+Lemma norm_bind_ex_l_conv : forall A fk1 fk, entails (@fex A (fun b => (bind (fk1 b) fk))) (bind (fex fk1) fk).
+Proof.
+Admitted.
+
+#[global]
+Instance Rewrite_binder_req : forall H f, RewritableBinder f -> RewritableBinder (req H f).
+Proof.
+  intros * H. inverts H. constructor. intros * Hf. apply rewritable_binder_proof0 in Hf.
+  rewrite norm_bind_req.
+  rewrite <- (norm_bind_req_conv _ _ f2).
+  apply entl_req_req; try xsimpl.
+  exact Hf.
+Qed.
+
+#[global]
+Instance Rewrite_binder_fall : forall A f, (forall v, RewritableBinder (f v)) -> RewritableBinder (@fall A f).
+Proof.
+  intros * H. constructor. intros * Hf.
+  (*apply rewritable_binder_proof0 in Hf.*)
+  Search (bind (fall _) _).
+  rewrite norm_bind_all_l.
+  rewrite <- (norm_bind_all_l_conv _ _ f2).
+  apply entl_all_r. intros b.
+  apply entl_all_l. exists b.
+  pose proof (H b).
+  inverts H0.
+  apply rewritable_binder_proof0.
+  exact Hf.
+Qed.
+
+#[global]
+Instance Rewrite_binder_fex : forall A f, (forall v, RewritableBinder (f v)) -> RewritableBinder (@fex A f).
+Proof.
+  intros * H. constructor. intros * Hf.
+  (*apply rewritable_binder_proof0 in Hf.*)
+  Search (bind (fall _) _).
+  rewrite norm_bind_ex_l.
+  rewrite <- (norm_bind_ex_l_conv _ _ f2).
+  fdestruct b. fexists b.
+  pose proof (H b).
+  inverts H0.
+  apply rewritable_binder_proof0.
+  exact Hf.
+Qed.
+
 #[global]
 Instance Proper_bind_t_entails_l : 
   forall A I,
@@ -454,64 +725,67 @@ Qed.
 
 #[global]
 Instance Proper_bind_t_entails_r :
-  forall A I f, ShiftFree f ->
+  forall A I f, RewritableBinder f ->
   Proper ((Morphisms.pointwise_relation _ entails) ====> entails) (@bind_t A I f).
 Proof.
   unfold Proper, respectful, Morphisms.pointwise_relation, bind_t.
   intros * Hent * Hpointwise.
-  setoid_rewrite Hpointwise.
-  reflexivity.
+  inverts Hent.
+  apply rewritable_binder_proof0. intros v.
+  fdestruct v_typed. fexists v_typed.
+  apply entails_ens_seq; try (xsimpl; auto).
+  apply Hpointwise.
 Qed.
 
-
-#[global]
-Instance Proper_bind_t_bientails_l : 
-  forall A I,
-  Proper (bientails ====> eq ====> bientails) (@bind_t A I).
-Proof.
-  unfold Proper, respectful, Morphisms.pointwise_relation, bind_t.
-  intros * Hbient * Hpointwise_bient.
-  apply bientails_iff_entails.
-  apply bientails_iff_entails in Hbient.
-  destruct Hbient as [Hxy Hyx].
-  subst.
-  split.
-  - setoid_rewrite Hxy. reflexivity.
-  - setoid_rewrite Hyx. reflexivity.
-Qed.
-
-#[global]
-Instance Proper_bind_t_bientails_r :
-  forall A I f,
-  ShiftFree f ->
-  Proper ((Morphisms.pointwise_relation _ bientails) ====> bientails) (@bind_t A I f).
-Proof.
-  unfold Proper, respectful, Morphisms.pointwise_relation, bind_t.
-  intros * Hsf * Hpointwise_bient.
-  apply bientails_iff_entails.
-  setoid_rewrite bientails_iff_entails in Hpointwise_bient.
-  apply forall_conj_inv_1 in Hpointwise_bient.
-  destruct Hpointwise_bient as [Hxy Hyx].
-  split.
-  - Search (bind _ (fun _ => fex _)).
-    rewrite norm_bind_ex_r. 2: { exact shift_free_pf. }
-    fdestruct v_typed.
-
-    rewrite <- entailsR_is_entails.
-    rewrite norm_bind_ex_r. 2: { exact shift_free_pf. }
-    rewrite entailsR_is_entails.
-    fexists v_typed.
-    
-    setoid_rewrite Hxy.
-    reflexivity.
-  - rewrite norm_bind_ex_r. 2: { exact shift_free_pf. }
-    fdestruct v_typed.
-
-    rewrite <- entailsR_is_entails.
-    rewrite norm_bind_ex_r. 2: { exact shift_free_pf. }
-    rewrite entailsR_is_entails.
-    fexists v_typed.
-    
-    setoid_rewrite Hyx.
-    reflexivity.
-Qed.
+(**)
+(*#[global]*)
+(*Instance Proper_bind_t_bientails_l : *)
+(*  forall A I,*)
+(*  Proper (bientails ====> eq ====> bientails) (@bind_t A I).*)
+(*Proof.*)
+(*  unfold Proper, respectful, Morphisms.pointwise_relation, bind_t.*)
+(*  intros * Hbient * Hpointwise_bient.*)
+(*  apply bientails_iff_entails.*)
+(*  apply bientails_iff_entails in Hbient.*)
+(*  destruct Hbient as [Hxy Hyx].*)
+(*  subst.*)
+(*  split.*)
+(*  - setoid_rewrite Hxy. reflexivity.*)
+(*  - setoid_rewrite Hyx. reflexivity.*)
+(*Qed.*)
+(**)
+(*#[global]*)
+(*Instance Proper_bind_t_bientails_r :*)
+(*  forall A I f,*)
+(*  ShiftFree f ->*)
+(*  Proper ((Morphisms.pointwise_relation _ bientails) ====> bientails) (@bind_t A I f).*)
+(*Proof.*)
+(*  unfold Proper, respectful, Morphisms.pointwise_relation, bind_t.*)
+(*  intros * Hsf * Hpointwise_bient.*)
+(*  apply bientails_iff_entails.*)
+(*  setoid_rewrite bientails_iff_entails in Hpointwise_bient.*)
+(*  apply forall_conj_inv_1 in Hpointwise_bient.*)
+(*  destruct Hpointwise_bient as [Hxy Hyx].*)
+(*  split.*)
+(*  - Search (bind _ (fun _ => fex _)).*)
+(*    rewrite norm_bind_ex_r. 2: { exact shift_free_pf. }*)
+(*    fdestruct v_typed.*)
+(**)
+(*    rewrite <- entailsR_is_entails.*)
+(*    rewrite norm_bind_ex_r. 2: { exact shift_free_pf. }*)
+(*    rewrite entailsR_is_entails.*)
+(*    fexists v_typed.*)
+(**)
+(*    setoid_rewrite Hxy.*)
+(*    reflexivity.*)
+(*  - rewrite norm_bind_ex_r. 2: { exact shift_free_pf. }*)
+(*    fdestruct v_typed.*)
+(**)
+(*    rewrite <- entailsR_is_entails.*)
+(*    rewrite norm_bind_ex_r. 2: { exact shift_free_pf. }*)
+(*    rewrite entailsR_is_entails.*)
+(*    fexists v_typed.*)
+(**)
+(*    setoid_rewrite Hyx.*)
+(*    reflexivity.*)
+(*Qed.*)
